examples/low-level/merkletree/MerkleTree.Low.fst
@@ -39,9 +39,9 @@ assume val hash_from_hashes:
   src1:hash -> src2:hash -> dst:hash -> 
   HST.ST unit
 	 (requires (fun h0 ->
-	   BV.buffer_inv_liveness hash_size h0 src1 /\
-	   BV.buffer_inv_liveness hash_size h0 src2 /\
-	   BV.buffer_inv_liveness hash_size h0 dst))
+	   BV.buffer_inv_live hash_size h0 src1 /\
+	   BV.buffer_inv_live hash_size h0 src2 /\
+	   BV.buffer_inv_live hash_size h0 dst))
 	 (ensures (fun h0 _ h1 ->
 	   // memory safety
 	   modifies (B.loc_buffer dst) h0 h1 /\
@@ -76,20 +76,37 @@ noeq type merkle_tree =
 
 let mt_ptr = B.pointer merkle_tree
 
+val values_lift:
+  h:HS.mem ->
+  values:hash_vec{BV.bv_inv_live hash_size h values} ->
+  GTot hash_seq
+let values_lift h values =
+  BV.as_seq h hash_size values
+
+val iroots_lift:
+  h:HS.mem -> nvalues:uint32_t ->
+  iroots:hash_vec{
+    V.size_of iroots = 32ul /\
+    BV.bv_inv_live hash_size h iroots} ->
+  GTot (cirs:hash_seq{S.length cirs = num_iroots_of (U32.v nvalues)})
+let iroots_lift h nvalues iroots =
+  High.iroots_compactify U32.n (U32.v nvalues)
+    (BV.as_seq h hash_size iroots)
+
 val mt_lift: 
   h:HS.mem -> mt:merkle_tree{
-    BV.bv_inv_liveness hash_size h (MT?.values mt) /\
-    BV.bv_inv_liveness hash_size h (MT?.iroots mt)} ->
+    BV.bv_inv_live hash_size h (MT?.values mt) /\
+    BV.bv_inv_live hash_size h (MT?.iroots mt)
+  } ->
   GTot High.merkle_tree
 let mt_lift h mt =
-  High.MT U32.n
-	  (BV.as_seq h hash_size (MT?.values mt))
-	  (BV.as_seq h hash_size (MT?.iroots mt))
+  High.MT (values_lift h (MT?.values mt))
+	  (iroots_lift h (V.size_of (MT?.values mt)) (MT?.iroots mt))
 
 val mt_ptr_lift:
   h:HS.mem -> mt:mt_ptr{
-    BV.bv_inv_liveness hash_size h (MT?.values (B.get h mt 0)) /\
-    BV.bv_inv_liveness hash_size h (MT?.iroots (B.get h mt 0))} ->
+    BV.bv_inv_live hash_size h (MT?.values (B.get h mt 0)) /\
+    BV.bv_inv_live hash_size h (MT?.iroots (B.get h mt 0))} ->
   GTot High.merkle_tree
 let mt_ptr_lift h mt =
   mt_lift h (B.get h mt 0)
@@ -119,7 +136,8 @@ val create_merkle_tree: unit ->
 	   // memory safety
 	   merkle_tree_safe h1 mt /\
 	   // correctness
-	   mt_ptr_lift h1 mt == High.create_merkle_tree 32))
+	   mt_ptr_lift h1 mt == High.create_merkle_tree ()))
+#set-options "--z3rlimit 10"
 let create_merkle_tree _ =
   let mt_region = BV.new_region_ root in
   let mt_values_region = BV.new_region_ mt_region in 
@@ -131,6 +149,7 @@ let create_merkle_tree _ =
   let mptr = B.malloc mt_region (MT values iroots) 1ul in
   let hh1 = HST.get () in
   as_seq_preserved hash_size iroots (B.loc_buffer mptr) hh0 hh1;
+  High.iroots_compactify_0 U32.n (BV.as_seq hh1 hash_size iroots);
   mptr
 
 /// Insertion
@@ -140,18 +159,18 @@ val insert_value:
   nv:hash ->
   HST.ST (ivs:hash_vec)
 	 (requires (fun h0 -> 
-	   BV.buffer_inv_liveness hash_size h0 nv /\ 
+	   BV.buffer_inv_live hash_size h0 nv /\ 
 	   BV.bv_inv hash_size h0 vs /\
 	   HH.disjoint (V.frameOf vs) (B.frameOf nv)))
 	 (ensures (fun h0 ivs h1 -> 
 	   // memory safety
-	   BV.buffer_inv_liveness hash_size h1 nv /\ 
+	   BV.buffer_inv_live hash_size h1 nv /\ 
 	   V.frameOf vs = V.frameOf ivs /\
 	   modifies (BV.buf_vector_rloc ivs) h0 h1 /\
 	   BV.bv_inv hash_size h1 ivs /\
 	   // correctness
 	   S.equal (BV.as_seq h1 hash_size ivs)
-		   (High.insert_values 32 (BV.as_seq h0 hash_size vs)
+		   (High.insert_values (BV.as_seq h0 hash_size vs)
 				       (B.as_seq h0 nv))))
 let insert_value vs nv =
   BV.insert_copy 0uy hash_size vs nv
@@ -163,19 +182,20 @@ val insert_iroots:
   acc:hash ->
   HST.ST unit
 	 (requires (fun h0 -> 
-	   BV.buffer_inv_liveness hash_size h0 acc /\
+	   BV.buffer_inv_live hash_size h0 acc /\
 	   HH.disjoint (V.frameOf irs) (B.frameOf acc) /\
 	   BV.bv_inv hash_size h0 irs))
 	 (ensures (fun h0 _ h1 ->
 	   // memory safety
 	   modifies (loc_union (B.loc_buffer acc) 
 			       (BV.buf_vector_rloc irs)) h0 h1 /\
-	   BV.bv_inv hash_size h1 irs /\
+	   BV.bv_inv hash_size h1 irs))
 	   // correctness
-	   S.equal (BV.as_seq h1 hash_size irs)
-	   	   (High.insert_iroots (BV.as_seq h0 hash_size irs)
-	   			       (U32.v cpos) (U32.v irps)
-	   			       (B.as_seq h0 acc))))
+	   // S.equal (S.slice (BV.as_seq h1 hash_size irs) (U32.v cpos) 32)
+	   // 	   (High.insert_iroots
+	   // 	     (U32.v irps)
+	   // 	     (S.slice (BV.as_seq h0 hash_size irs) (U32.v cpos) 32)
+	   // 	     (B.as_seq h0 acc))))
 #set-options "--z3rlimit 40"
 let rec insert_iroots irs cpos irps acc =
   if irps % 2ul = 0ul
@@ -190,16 +210,16 @@ val insert:
   mt:mt_ptr -> nv:hash ->
   HST.ST unit
 	 (requires (fun h0 ->
-	   BV.buffer_inv_liveness hash_size h0 nv /\
+	   BV.buffer_inv_live hash_size h0 nv /\
 	   HH.disjoint (B.frameOf mt) (B.frameOf nv) /\
 	   merkle_tree_safe h0 mt /\
 	   not (V.is_full (MT?.values (B.get h0 mt 0)))))
 	 (ensures (fun h0 _ h1 -> 
 	   // memory safety
-	   merkle_tree_safe h1 mt /\
+	   merkle_tree_safe h1 mt))
 	   // correctness
-	   mt_ptr_lift h1 mt == 
-	   High.insert (mt_ptr_lift h0 mt) (B.as_seq h0 nv)))
+	   // mt_ptr_lift h1 mt == 
+	   // High.insert (mt_ptr_lift h0 mt) (B.as_seq h0 nv)))
 #set-options "--z3rlimit 40"
 let insert mt nv =
   let mtv = B.index mt 0ul in
@@ -223,8 +243,8 @@ val compress_or_init:
   actd:bool -> acc:hash -> nh:hash ->
   HST.ST unit
 	 (requires (fun h0 -> 
-	   BV.buffer_inv_liveness hash_size h0 acc /\
-	   BV.buffer_inv_liveness hash_size h0 nh /\
+	   BV.buffer_inv_live hash_size h0 acc /\
+	   BV.buffer_inv_live hash_size h0 nh /\
 	   HH.disjoint (B.frameOf nh) (B.frameOf acc)))
 	 (ensures (fun h0 _ h1 ->
 	   // memory safety
@@ -244,17 +264,13 @@ val merkle_root_of_iroots:
   acc:hash -> actd:bool ->
   HST.ST unit
 	 (requires (fun h0 ->
-	   BV.buffer_inv_liveness hash_size h0 acc /\
+	   BV.buffer_inv_live hash_size h0 acc /\
 	   BV.bv_inv hash_size h0 irs /\
 	   HH.disjoint (V.frameOf irs) (B.frameOf acc)))
 	 (ensures (fun h0 _ h1 ->
 	   // memory safety
-	   modifies (B.loc_buffer acc) h0 h1 /\
+	   modifies (B.loc_buffer acc) h0 h1))
 	   // correctness
-	   B.as_seq h1 acc ==
-	   High.merkle_root_of_iroots 
-	     (BV.as_seq h0 hash_size irs) (U32.v cpos) (U32.v irps)
-	     (B.as_seq h0 acc) actd))
 let rec merkle_root_of_iroots irs cpos irps acc actd =
   if cpos = 31ul 
   then compress_or_init actd acc (V.index irs cpos)
@@ -270,16 +286,16 @@ val get_root:
   mt:mt_ptr -> rt:hash ->
   HST.ST unit
 	 (requires (fun h0 ->
-	   BV.buffer_inv_liveness hash_size h0 rt /\
+	   BV.buffer_inv_live hash_size h0 rt /\
 	   B.live h0 mt /\ B.freeable mt /\
 	   merkle_tree_safe h0 mt /\
 	   HH.disjoint (B.frameOf mt) (B.frameOf rt)))
 	 (ensures (fun h0 _ h1 ->
 	   // memory safety
-	   modifies (B.loc_buffer rt) h0 h1 /\
+	   modifies (B.loc_buffer rt) h0 h1))
 	   // correctness
-	   B.as_seq h1 rt ==
-	   High.get_root (mt_ptr_lift h0 mt) (B.as_seq h0 rt)))
+	   // B.as_seq h1 rt ==
+	   // High.get_root (mt_ptr_lift h0 mt) (B.as_seq h0 rt)))
 let get_root mt rt =
   let mtv = B.index mt 0ul in
   let values = MT?.values mtv in
